compiler/eval/compilerComputeLib.sml
@@ -343,6 +343,7 @@ in
     ,bvp_to_wordTheory.adjust_set_def
     ,bvp_to_wordTheory.Unit_def
     ,bvp_to_wordTheory.GiveUp_def
+    ,bvp_to_wordTheory.make_header_def
     ,bvp_to_wordTheory.encode_header_def
     ,bvp_to_wordTheory.list_Seq_def
     ,bvp_to_wordTheory.shift_def
